semantics/alt_semantics/proofs/bigSmallEquivScript.sml
@@ -447,13 +447,13 @@ val (small_eval_match_rules, small_eval_match_ind, small_eval_match_cases) = Hol
 (!env s err_v v. small_eval_match env s v [] err_v (s, Rerr (Rraise err_v))) ∧
 (!env s p e pes r v err_v.
   ALL_DISTINCT (pat_bindings p []) ∧
-  pmatch env.c (FST s) p v env.v = Match env' ∧
-  small_eval (env with v := env') s e [] r
+  pmatch env.c (FST s) p v [] = Match env' ∧
+  small_eval (env with v := eAppend (alist_to_env env') env.v) s e [] r
   ⇒
   small_eval_match env s v ((p,e)::pes) err_v r) ∧
 (!env s e p pes r v err_v.
   ALL_DISTINCT (pat_bindings p []) ∧
-  (pmatch env.c (FST s) p v env.v = No_match) ∧
+  (pmatch env.c (FST s) p v [] = No_match) ∧
   small_eval_match env s v pes err_v r
   ⇒
   small_eval_match env s v ((p,e)::pes) err_v r) ∧
@@ -462,7 +462,7 @@ val (small_eval_match_rules, small_eval_match_ind, small_eval_match_cases) = Hol
   ⇒
   small_eval_match env s v ((p,e)::pes) err_v (s, Rerr (Rabort Rtype_error))) ∧
 (!env s p e pes v err_v.
-  (pmatch env.c (FST s) p v env.v = Match_type_error)
+  (pmatch env.c (FST s) p v [] = Match_type_error)
   ⇒
   small_eval_match env s v ((p,e)::pes) err_v (s, Rerr (Rabort Rtype_error)))`;
 
@@ -1140,11 +1140,11 @@ val big_exp_to_small_exp = Q.prove (
                       (env',to_small_st s',Val v,[(Clet n () e',env)])`
                by metis_tac [e_step_add_ctxt, APPEND] >>
        `e_step_reln (env',to_small_st s',Val v,[(Clet n () e',env)])
-                    (env with v := opt_bind n v env.v,to_small_st s',Exp e',[])`
+                    (env with v := eOptBind n v env.v,to_small_st s',Exp e',[])`
                by srw_tac[][e_step_def, e_step_reln_def, continue_def, push_def] >>
        Q.ISPEC_THEN`r`assume_tac result_cases >>
-       full_simp_tac(srw_ss())[small_eval_def, environment_component_equality] >>
-       full_simp_tac(srw_ss())[small_eval_def, environment_component_equality] >>
+       full_simp_tac(srw_ss())[small_eval_def, sem_env_component_equality] >>
+       full_simp_tac(srw_ss())[small_eval_def, sem_env_component_equality] >>
        metis_tac [transitive_RTC, RTC_SINGLE, transitive_def])
    >- (`small_eval env (to_small_st s) e ([] ++ [(Clet n () e2,env)]) (to_small_st s', Rerr err)`
                by (match_mp_tac small_eval_err_add_ctxt >>
